src/BS.v
@@ -2,12 +2,11 @@
    BS stands for "Binary String".  May be instantiated with 
    types like strings and byte buffers in concrete implementations.    *)
 
-Require Import String ResultT. 
+Require Import ResultT Serializable. 
 
 Definition BS : Set. Admitted.
 
-Definition BS_to_string (bs:BS) : string. Admitted.
-Definition string_to_BS (s: string) : ResultT BS string. Admitted.
+Global Instance Serializable_BS : Serializable BS. Admitted.
 
 (* Some default/reserved BS values *)
 Definition default_bs : BS. Admitted.
