src/CvmJson_Interfaces.v
@@ -3,102 +3,108 @@
     
     At the moment, these are too low-level to represent faithfully in the Coq development.   *)
 
-Require Import Term_Defs_Core Term_Defs String List JSON Interface_Types ResultT ErrorStringConstants Term_Defs_Admits BS.
+Require Import Term_Defs_Core Term_Defs List JSON Interface_Types ResultT ErrorStringConstants BS Serializable.
 Export Interface_Types JSON.
 Import ListNotations ResultNotation.
 
 (* Protocol Run Section *)
 Definition ProtocolRunRequest_to_JSON (req: ProtocolRunRequest): JSON :=
   JSON_Object 
-    [(STR_TYPE, (JSON_String STR_REQUEST));
-    (STR_ACTION, (JSON_String STR_RUN));
-    (STR_REQ_PLC, (JSON_String (Plc_to_string (prreq_req_plc req))));
-    (STR_TERM, (JSON_String (Term_to_string (prreq_term req)))); 
-    (STR_EV, (JSON_String (RawEv_to_string (prreq_ev req))))].
+    [(STR_TYPE, (InJSON_String STR_REQUEST));
+    (STR_ACTION, (InJSON_String STR_RUN));
+    (STR_REQ_PLC, (InJSON_String (to_string (prreq_req_plc req))));
+    (STR_TERM, (InJSON_Object (to_JSON (prreq_term req)))); 
+    (STR_EV, (InJSON_Object (to_JSON (prreq_ev req))))].
 
 Definition JSON_to_ProtocolRunRequest (req : JSON): ResultT ProtocolRunRequest string :=
-  temp_term <- JSON_get_string STR_TERM req ;;
+  temp_term <- JSON_get_Object STR_TERM req ;;
   temp_req_plc <- JSON_get_string STR_REQ_PLC req ;;
-  temp_ev <- JSON_get_string STR_EV req ;;
-  term <- string_to_Term temp_term ;;
-  req_plc <- string_to_Plc temp_req_plc ;;
-  ev <- string_to_RawEv temp_ev ;;
+  temp_ev <- JSON_get_Object STR_EV req ;;
+
+  term <- from_JSON temp_term ;;
+  req_plc <- from_string temp_req_plc ;;
+  ev <- from_JSON temp_ev ;;
   resultC (mkPRReq term req_plc ev).
 
 Definition ProtocolRunResponse_to_JSON (resp: ProtocolRunResponse): JSON :=
   JSON_Object 
-    [(STR_TYPE, (JSON_String STR_RESPONSE));
-    (STR_ACTION, (JSON_String STR_RUN));
-    (STR_SUCCESS, (JSON_Boolean (prresp_success resp)));
-    (STR_PAYLOAD, (JSON_String (RawEv_to_string (prresp_ev resp))))].
+    [(STR_TYPE, (InJSON_String STR_RESPONSE));
+    (STR_ACTION, (InJSON_String STR_RUN));
+    (STR_SUCCESS, (InJSON_Boolean (prresp_success resp)));
+    (STR_PAYLOAD, (InJSON_Object (to_JSON (prresp_ev resp))))].
 
 Definition JSON_to_ProtocolRunResponse (resp : JSON): ResultT ProtocolRunResponse string :=
   temp_success <- JSON_get_bool STR_SUCCESS resp ;;
-  temp_ev <- JSON_get_string STR_PAYLOAD resp ;;
-  ev <- string_to_RawEv temp_ev ;;
+  temp_ev <- JSON_get_Object STR_PAYLOAD resp ;;
+
+  ev <- from_JSON temp_ev ;;
   resultC (mkPRResp temp_success ev).
 
 (* Protocol Negotiate Section *)
 Definition ProtocolNegotiateRequest_to_JSON (req: ProtocolNegotiateRequest): JSON :=
-  JSON_Object 
-    [(STR_TYPE, (JSON_String STR_REQUEST));
-    (STR_ACTION, (JSON_String STR_NEGOTIATE));
-      (STR_TERM, (JSON_String (Term_to_string (pnreq_term req))))].
+  JSON_Object [
+    (STR_TYPE, (InJSON_String STR_REQUEST));
+    (STR_ACTION, (InJSON_String STR_NEGOTIATE)); 
+    (STR_TERM, (InJSON_Object (to_JSON (pnreq_term req))))
+  ].
 
-Definition JSON_to_ProtocolNegotiateRequest (req : JSON): 
-    ResultT ProtocolNegotiateRequest string :=
-  temp_term <- JSON_get_string STR_TERM req ;;
-  term <- string_to_Term temp_term ;;
+Definition JSON_to_ProtocolNegotiateRequest (req : JSON): ResultT ProtocolNegotiateRequest string :=
+  temp_term <- JSON_get_Object STR_TERM req ;;
+
+  term <- from_JSON temp_term ;;
   resultC (mkPNReq term).
 
 Definition ProtocolNegotiateResponse_to_JSON (resp: ProtocolNegotiateResponse): JSON :=
-  JSON_Object 
-    [(STR_TYPE, (JSON_String STR_RESPONSE));
-    (STR_ACTION, (JSON_String STR_NEGOTIATE));
-      (STR_SUCCESS, (JSON_Boolean (pnresp_success resp)));
-    (STR_PAYLOAD, (JSON_String (Term_to_string (pnresp_term resp))))].
+  JSON_Object [
+    (STR_TYPE, (InJSON_String STR_RESPONSE));
+    (STR_ACTION, (InJSON_String STR_NEGOTIATE)); 
+    (STR_SUCCESS, (InJSON_Boolean (pnresp_success resp)));
+    (STR_PAYLOAD, (InJSON_Object (to_JSON (pnresp_term resp))))
+  ].
 
-Definition JSON_to_ProtocolNegotiateResponse (resp : JSON): 
-    ResultT ProtocolNegotiateResponse string :=
+Definition JSON_to_ProtocolNegotiateResponse (resp : JSON): ResultT ProtocolNegotiateResponse string :=
   temp_success <- JSON_get_bool STR_SUCCESS resp ;;
-  temp_term <- JSON_get_string STR_PAYLOAD resp ;;
-  term <- string_to_Term temp_term ;;
+  temp_term <- JSON_get_Object STR_PAYLOAD resp ;;
+
+  term <- from_JSON temp_term ;;
   resultC (mkPNResp temp_success term).
 
 (* Protocol Appraise Section *)
 Definition ProtocolAppraiseRequest_to_JSON (req: ProtocolAppraiseRequest): JSON :=
-  JSON_Object 
-    [(STR_TYPE, (JSON_String STR_REQUEST));
-    (STR_ACTION, (JSON_String STR_APPRAISE));
-    (STR_TERM, (JSON_String (Term_to_string (pareq_term req))));
-    (STR_REQ_PLC, (JSON_String (Plc_to_string (pareq_plc req))));
-    (STR_EVIDENCE, (JSON_String (Evidence_to_string (pareq_evidence req))));
-    (STR_EV, (JSON_String (RawEv_to_string (pareq_ev req))))].
+  JSON_Object [
+    (STR_TYPE, (InJSON_String STR_REQUEST));
+    (STR_ACTION, (InJSON_String STR_APPRAISE));
+    (STR_TERM, (InJSON_Object (to_JSON (pareq_term req))));
+    (STR_REQ_PLC, (InJSON_String (to_string (pareq_plc req))));
+    (STR_EVIDENCE, (InJSON_Object (to_JSON (pareq_evidence req))));
+    (STR_EV, (InJSON_Object (to_JSON (pareq_ev req))))].
 
-Definition JSON_to_ProtocolAppraiseRequest (req : JSON): 
-    ResultT ProtocolAppraiseRequest string :=
-  temp_term <- JSON_get_string STR_TERM req ;;
+Definition JSON_to_ProtocolAppraiseRequest (req : JSON): ResultT ProtocolAppraiseRequest string :=
+  temp_term <- JSON_get_Object STR_TERM req ;;
   temp_plc <- JSON_get_string STR_REQ_PLC req ;;
-  temp_evidence <- JSON_get_string STR_EVIDENCE req ;;
-  temp_ev <- JSON_get_string STR_EV req ;;
-  term <- string_to_Term temp_term ;;
-  plc <- string_to_Plc temp_plc ;;
-  evidence <- string_to_Evidence temp_evidence ;;
-  ev <- string_to_RawEv temp_ev ;;
+  temp_evidence <- JSON_get_Object STR_EVIDENCE req ;;
+  temp_ev <- JSON_get_Object STR_EV req ;;
+
+  term <- from_JSON temp_term ;;
+  plc <- from_string temp_plc ;;
+  evidence <- from_JSON temp_evidence ;;
+  ev <- from_JSON temp_ev ;;
   resultC (mkPAReq term plc evidence ev).
 
 Definition ProtocolAppraiseResponse_to_JSON (resp: ProtocolAppraiseResponse): JSON :=
-  JSON_Object 
-    [(STR_TYPE, (JSON_String STR_RESPONSE));
-    (STR_ACTION, (JSON_String STR_APPRAISE));
-    (STR_SUCCESS, (JSON_Boolean (paresp_success resp)));
-    (STR_PAYLOAD, (JSON_String (AppResultC_to_string (paresp_result resp))))].
+  JSON_Object [
+    (STR_TYPE, (InJSON_String STR_RESPONSE));
+    (STR_ACTION, (InJSON_String STR_APPRAISE));
+    (STR_SUCCESS, (InJSON_Boolean (paresp_success resp)));
+    (STR_PAYLOAD, (InJSON_Object (to_JSON (paresp_result resp))))
+  ].
 
 Definition JSON_to_ProtocolAppraiseResponse (resp : JSON): 
     ResultT ProtocolAppraiseResponse string :=
   temp_success <- JSON_get_bool STR_SUCCESS resp ;;
-  temp_result <- JSON_get_string STR_PAYLOAD resp ;;
-  result <- string_to_AppResultC temp_result ;;
+  temp_result <- JSON_get_Object STR_PAYLOAD resp ;;
+
+  result <- from_JSON temp_result ;;
   resultC (mkPAResp temp_success result).
 
 (* AM Protocol Request Section *)
@@ -166,39 +172,42 @@ Definition JSON_to_AM_Protocol_Interface (msg : JSON):
 
 (* ASP Run Request Section *)
 Definition ASPRunRequest_to_JSON (req: ASPRunRequest): JSON :=
-  JSON_Object 
-    [(STR_TYPE, (JSON_String STR_REQUEST));
-    (STR_ACTION, (JSON_String STR_ASP_RUN));
-    (STR_ASP_ID, (JSON_String (ASP_ID_to_string (asprreq_asp_id req))));
-    (STR_ASP_ARGS, (JSON_String (ASP_ARGS_to_string (asprreq_asp_args req))));
-    (STR_TARG_PLC, (JSON_String (Plc_to_string (asprreq_targ_plc req))));
-    (STR_TARG, (JSON_String (TARG_ID_to_string (asprreq_targ req))));
-    (STR_EV, (JSON_String (RawEv_to_string (asprreq_rawev req))))].
+  JSON_Object [
+    (STR_TYPE, (InJSON_String STR_REQUEST));
+    (STR_ACTION, (InJSON_String STR_ASP_RUN));
+    (STR_ASP_ID, (InJSON_String (to_string (asprreq_asp_id req))));
+    (STR_ASP_ARGS, (InJSON_Object (to_JSON (asprreq_asp_args req))));
+    (STR_TARG_PLC, (InJSON_String (to_string (asprreq_targ_plc req))));
+    (STR_TARG, (InJSON_String (to_string (asprreq_targ req))));
+    (STR_EV, (InJSON_Object (to_JSON (asprreq_rawev req))))
+  ].
 
 Definition JSON_to_ASPRunRequest (req : JSON): ResultT ASPRunRequest string :=
   temp_asp_id <- JSON_get_string STR_ASP_ID req ;;
-  temp_asp_args <- JSON_get_string STR_ASP_ARGS req ;;
+  temp_asp_args <- JSON_get_Object STR_ASP_ARGS req ;;
   temp_targ_plc <- JSON_get_string STR_TARG_PLC req ;;
   temp_targ <- JSON_get_string STR_TARG req ;;
-  temp_ev <- JSON_get_string STR_EV req ;;
-  asp_id <- string_to_ASP_ID temp_asp_id ;;
-  asp_args <- string_to_ASP_ARGS temp_asp_args ;;
-  targ_plc <- string_to_Plc temp_targ_plc ;;
-  targ <- string_to_TARG_ID temp_targ ;;
-  ev <- string_to_RawEv temp_ev ;;
+  temp_ev <- JSON_get_Object STR_EV req ;;
+
+  asp_id <- from_string temp_asp_id ;;
+  asp_args <- from_JSON temp_asp_args ;;
+  targ_plc <- from_string temp_targ_plc ;;
+  targ <- from_string temp_targ ;;
+  ev <- from_JSON temp_ev ;;
   resultC (mkASPRReq asp_id asp_args targ_plc targ ev).
 
 Definition ASPRunResponse_to_JSON (resp: ASPRunResponse): JSON :=
   JSON_Object 
-    [(STR_TYPE, (JSON_String STR_RESPONSE));
-    (STR_ACTION, (JSON_String STR_ASP_RUN));
-    (STR_SUCCESS, (JSON_Boolean (asprresp_success resp)));
-    (STR_PAYLOAD, (JSON_String (RawEv_to_string (asprresp_rawev resp))))].
+    [(STR_TYPE, (InJSON_String STR_RESPONSE));
+    (STR_ACTION, (InJSON_String STR_ASP_RUN));
+    (STR_SUCCESS, (InJSON_Boolean (asprresp_success resp)));
+    (STR_PAYLOAD, (InJSON_Object (to_JSON (asprresp_rawev resp))))].
 
 Definition JSON_to_ASPRunResponse (resp : JSON): ResultT ASPRunResponse string :=
   temp_success <- JSON_get_bool STR_SUCCESS resp ;;
-  temp_rawev <- JSON_get_string STR_PAYLOAD resp ;;
-  rawev <- string_to_RawEv temp_rawev ;;
+  temp_rawev <- JSON_get_Object STR_PAYLOAD resp ;;
+
+  rawev <- from_JSON temp_rawev ;;
   resultC (mkASPRResp temp_success rawev).
 
 (* AM ASP Interface Section *)
@@ -228,5 +237,5 @@ Definition JSON_to_AM_ASP_Interface (msg : JSON):
 (* Error Response *)
 Definition ErrorResponseJSON (msg: string): JSON :=
   JSON_Object 
-    [(STR_SUCCESS, JSON_Boolean false);
-    (STR_PAYLOAD, (JSON_String msg))].
+    [(STR_SUCCESS, InJSON_Boolean false);
+    (STR_PAYLOAD, (InJSON_String msg))].
